{-# OPTIONS --without-K --exact-split --safe #-}

module HoTT-UF-Agda where

open import Universes
open import MLTT-Agda

is-subsingleton : 𝓤 ̇ → 𝓤 ̇
is-subsingleton X = (x y : X) → x ≡ y

𝟘-is-subsingleton : is-subsingleton 𝟘
𝟘-is-subsingleton x y = !𝟘 (x ≡ y) x

𝟙-is-subsingleton : is-subsingleton 𝟙
𝟙-is-subsingleton = 𝟙-induction (λ x → ∀ y → x ≡ y) (𝟙-induction (λ y → ⋆ ≡ y) (refl ⋆))

𝟙-is-subsingleton' : is-subsingleton 𝟙
𝟙-is-subsingleton' ⋆ ⋆  = refl ⋆

is-prop is-truth-value : 𝓤 ̇ → 𝓤 ̇
is-prop        = is-subsingleton
is-truth-value = is-subsingleton

is-set : 𝓤 ̇ → 𝓤 ̇
is-set X = (x y : X) → is-subsingleton (x ≡ y)

Magma : (𝓤 : Universe) → 𝓤 ⁺ ̇
Magma 𝓤 = Σ \(X : 𝓤 ̇ ) → is-set X × (X → X → X)

⟨_⟩ : Magma 𝓤 → 𝓤 ̇
⟨ X , i , _·_ ⟩ = X

magma-is-set : (M : Magma 𝓤) → is-set ⟨ M ⟩
magma-is-set (X , i , _·_) = i

magma-operation : (M : Magma 𝓤) → ⟨ M ⟩ → ⟨ M ⟩ → ⟨ M ⟩
magma-operation (X , i , _·_) = _·_

syntax magma-operation M x y = x ·⟨ M ⟩ y

is-magma-hom : (M N : Magma 𝓤) → (⟨ M ⟩ → ⟨ N ⟩) → 𝓤 ̇
is-magma-hom M N f = (x y : ⟨ M ⟩) → f (x ·⟨ M ⟩ y) ≡ f x ·⟨ N ⟩ f y

id-is-magma-hom : (M : Magma 𝓤) → is-magma-hom M M (𝑖𝑑 ⟨ M ⟩)
id-is-magma-hom M = λ (x y : ⟨ M ⟩) → refl (x ·⟨ M ⟩ y)

is-magma-iso : (M N : Magma 𝓤) → (⟨ M ⟩ → ⟨ N ⟩) → 𝓤 ̇
is-magma-iso M N f = is-magma-hom M N f
                   × Σ \(g : ⟨ N ⟩ → ⟨ M ⟩) → is-magma-hom N M g
                                            × (g ∘ f ∼ 𝑖𝑑 ⟨ M ⟩)
                                            × (f ∘ g ∼ 𝑖𝑑 ⟨ N ⟩)

id-is-magma-iso : (M : Magma 𝓤) → is-magma-iso M M (𝑖𝑑 ⟨ M ⟩)
id-is-magma-iso M = id-is-magma-hom M ,
                    𝑖𝑑 ⟨ M ⟩ ,
                    id-is-magma-hom M ,
                    refl ,
                    refl

⌜_⌝ : {M N : Magma 𝓤} → M ≡ N → ⟨ M ⟩ → ⟨ N ⟩
⌜ p ⌝ = transport ⟨_⟩ p

⌜⌝-is-iso : {M N : Magma 𝓤} (p : M ≡ N) → is-magma-iso M N (⌜ p ⌝)
⌜⌝-is-iso (refl M) = id-is-magma-iso M

_≅ₘ_ : Magma 𝓤 → Magma 𝓤 → 𝓤 ̇
M ≅ₘ N = Σ \(f : ⟨ M ⟩ → ⟨ N ⟩) → is-magma-iso M N f

magma-Id-to-iso : {M N : Magma 𝓤} → M ≡ N → M ≅ₘ N
magma-Id-to-iso p = (⌜ p ⌝ , ⌜⌝-is-iso p )

∞-Magma : (𝓤 : Universe) → 𝓤 ⁺ ̇
∞-Magma 𝓤 = Σ \(X : 𝓤 ̇ ) → X → X → X

left-neutral : {X : 𝓤 ̇ } → X → (X → X → X) → 𝓤 ̇
left-neutral e _·_ = ∀ x → e · x ≡ x

right-neutral : {X : 𝓤 ̇ } → X → (X → X → X) → 𝓤 ̇
right-neutral e _·_ = ∀ x → x · e ≡ x

associative : {X : 𝓤 ̇ } → (X → X → X) → 𝓤 ̇
associative _·_ = ∀ x y z → (x · y) · z ≡ x · (y · z)

Monoid : (𝓤 : Universe) → 𝓤 ⁺ ̇
Monoid 𝓤 = Σ \(X : 𝓤 ̇ ) → is-set X
                         × Σ \(_·_ : X → X → X)
                         → Σ \(e : X)
                         → left-neutral e _·_
                         × right-neutral e _·_
                         × associative _·_

refl-left : {X : 𝓤 ̇ } {x y : X} {p : x ≡ y} → refl x ∙ p ≡ p
refl-left {𝓤} {X} {x} {x} {refl x} = refl (refl x)

refl-right : {X : 𝓤 ̇ } {x y : X} {p : x ≡ y} → p ∙ refl y ≡ p
refl-right {𝓤} {X} {x} {y} {p} = refl p

∙assoc : {X : 𝓤 ̇ } {x y z t : X} (p : x ≡ y) (q : y ≡ z) (r : z ≡ t)
       → (p ∙ q) ∙ r ≡ p ∙ (q ∙ r)
∙assoc p q (refl z) = refl (p ∙ q)

⁻¹-left∙ : {X : 𝓤 ̇ } {x y : X} (p : x ≡ y)
         → p ⁻¹ ∙ p ≡ refl y
⁻¹-left∙ (refl x) = refl (refl x)

⁻¹-right∙ : {X : 𝓤 ̇ } {x y : X} (p : x ≡ y)
          → p ∙ p ⁻¹ ≡ refl x
⁻¹-right∙ (refl x) = refl (refl x)

⁻¹-involutive : {X : 𝓤 ̇ } {x y : X} (p : x ≡ y)
              → (p ⁻¹)⁻¹ ≡ p
⁻¹-involutive (refl x) = refl (refl x)

ap-refl : {X : 𝓤 ̇ } {Y : 𝓥 ̇ } (f : X → Y) (x : X)
        → ap f (refl x) ≡ refl (f x)
ap-refl f x = refl (refl (f x))

ap-∙ : {X : 𝓤 ̇ } {Y : 𝓥 ̇ } (f : X → Y) {x y z : X} (p : x ≡ y) (q : y ≡ z)
     → ap f (p ∙ q) ≡ ap f p ∙ ap f q
ap-∙ f p (refl y) = refl (ap f p)

ap-id : {X : 𝓤 ̇ } {x y : X} (p : x ≡ y)
      → ap id p ≡ p
ap-id (refl x) = refl (refl x)

ap-∘ : {X : 𝓤 ̇ } {Y : 𝓥 ̇ } {Z : 𝓦 ̇ }
       (f : X → Y) (g : Y → Z) {x y : X} (p : x ≡ y)
     → ap (g ∘ f) p ≡ (ap g ∘ ap f) p
ap-∘ f g (refl x) = refl (refl (g (f x)))

transport∙ : {X : 𝓤 ̇ } (A : X → 𝓥 ̇ ) {x y z : X} (p : x ≡ y) (q : y ≡ z)
           → transport A (p ∙ q) ≡ transport A q ∘ transport A p
transport∙ A p (refl y) = refl (transport A p)

Nat : {X : 𝓤 ̇ } → (X → 𝓥 ̇ ) → (X → 𝓦 ̇ ) → 𝓤 ⊔ 𝓥 ⊔ 𝓦 ̇
Nat A B = (x : domain A) → A x → B x

Nats-are-natural : {X : 𝓤 ̇ } (A : X → 𝓥 ̇ ) (B : X → 𝓦 ̇ ) (τ : Nat A B)
                 → {x y : X} (p : x ≡ y) → τ y ∘ transport A p ≡ transport B p ∘ τ x
Nats-are-natural A B τ (refl x) = refl (τ x)

NatΣ : {X : 𝓤 ̇ } {A : X → 𝓥 ̇ } {B : X → 𝓦 ̇ } → Nat A B → Σ A → Σ B
NatΣ τ (x , a) = (x , τ x a)

data Color : 𝓤₀ ̇  where
 Black White : Color

dId : {X : 𝓤 ̇ } (A : X → 𝓥 ̇ ) {x y : X} (p : x ≡ y) → A x → A y → 𝓥 ̇
dId A p a b = transport A p a ≡ b

syntax dId A p a b = a ≡[ p / A ] b

≡[]-on-refl-is-≡ : {X : 𝓤 ̇ } (A : X → 𝓥 ̇ ) {x : X} (a b : A x)
                 → (a ≡[ refl x / A ] b) ≡ (a ≡ b)
≡[]-on-refl-is-≡ A {x} a b = refl (a ≡ b)

≡[]-on-refl-is-≡' : {X : 𝓤 ̇ } (A : X → 𝓥 ̇ ) {x : X} (a b : A x)
                  → (a ≡[ refl x / A ] b) ≡ (a ≡ b)

≡[]-on-refl-is-≡' {𝓤} {𝓥} {X} A {x} a b = refl {𝓥 ⁺} {𝓥 ̇ } (a ≡ b)

to-Σ-≡ : {X : 𝓤 ̇ } {A : X → 𝓥 ̇ } {σ τ : Σ A}
       → (Σ \(p : pr₁ σ ≡ pr₁ τ) → pr₂ σ ≡[ p / A ] pr₂ τ)
       → σ ≡ τ
to-Σ-≡ (refl x , refl a) = refl (x , a)

from-Σ-≡ : {X : 𝓤 ̇ } {A : X → 𝓥 ̇ } {σ τ : Σ A}
         → σ ≡ τ
         → Σ \(p : pr₁ σ ≡ pr₁ τ) → pr₂ σ ≡[ p / A ] pr₂ τ
from-Σ-≡ (refl (x , a)) = (refl x , refl a)

is-singleton : 𝓤 ̇ → 𝓤 ̇
is-singleton X = Σ \(c : X) → (x : X) → c ≡ x

𝟙-is-singleton : is-singleton 𝟙
𝟙-is-singleton = ⋆ , 𝟙-induction (λ x → ⋆ ≡ x) (refl ⋆)

_is-of-hlevel_ : 𝓤 ̇ → ℕ → 𝓤 ̇
X is-of-hlevel 0        = is-singleton X
X is-of-hlevel (succ n) = (x x' : X) → ((x ≡ x') is-of-hlevel n)

center : (X : 𝓤 ̇ ) → is-singleton X → X
center X (c , φ) = c

centrality : (X : 𝓤 ̇ ) (i : is-singleton X) (x : X) → center X i ≡ x
centrality X (c , φ) = φ

singletons-are-subsingletons : (X : 𝓤 ̇ ) → is-singleton X → is-subsingleton X
singletons-are-subsingletons X (c , φ) x y = x ≡⟨ (φ x)⁻¹ ⟩
                                             c ≡⟨ φ y ⟩
                                             y ∎

pointed-subsingletons-are-singletons : (X : 𝓤 ̇ ) → X → is-subsingleton X → is-singleton X
pointed-subsingletons-are-singletons X x s = (x , s x)

EM EM' : ∀ 𝓤 → 𝓤 ⁺ ̇
EM  𝓤 = (X : 𝓤 ̇ ) → is-subsingleton X → X + ¬ X
EM' 𝓤 = (X : 𝓤 ̇ ) → is-subsingleton X → is-singleton X + is-empty X

EM-gives-EM' : EM 𝓤 → EM' 𝓤
EM-gives-EM' em X s = γ (em X s)
 where
  γ : X + ¬ X → is-singleton X + is-empty X
  γ (inl x) = inl (pointed-subsingletons-are-singletons X x s)
  γ (inr x) = inr x

EM'-gives-EM : EM' 𝓤 → EM 𝓤
EM'-gives-EM em' X s = γ (em' X s)
 where
  γ : is-singleton X + is-empty X → X + ¬ X
  γ (inl i) = inl (center X i)
  γ (inr x) = inr x

wconstant : {X : 𝓤 ̇ } {Y : 𝓥 ̇ } → (f : X → Y) → 𝓤 ⊔ 𝓥 ̇
wconstant f = (x x' : domain f) → f x ≡ f x'

collapsible : 𝓤 ̇ → 𝓤 ̇
collapsible X = Σ \(f : X → X) → wconstant f

collapser : (X : 𝓤 ̇ ) → collapsible X → X → X
collapser X (f , w) = f

collapser-wconstancy : (X : 𝓤 ̇ ) (c : collapsible X) → wconstant (collapser X c)
collapser-wconstancy X (f , w) = w

hedberg : {X : 𝓤 ̇ } (x : X)
        → ((y : X) → collapsible (x ≡ y))
        → (y : X) → is-subsingleton (x ≡ y)
hedberg {𝓤} {X} x c y p q =
 p                       ≡⟨ a y p ⟩
 f x (refl x)⁻¹ ∙ f y p  ≡⟨ ap (λ - → (f x (refl x))⁻¹ ∙ -) (κ y p q) ⟩
 f x (refl x)⁻¹ ∙ f y q  ≡⟨ (a y q)⁻¹ ⟩
 q                       ∎
 where
  f : (y : X) → x ≡ y → x ≡ y
  f y = collapser (x ≡ y) (c y)
  κ : (y : X) (p q : x ≡ y) → f y p ≡ f y q
  κ y = collapser-wconstancy (x ≡ y) (c y)
  a : (y : X) (p : x ≡ y) → p ≡ (f x (refl x))⁻¹ ∙ f y p
  a x (refl x) = (⁻¹-left∙ (f x (refl x)))⁻¹

≡-collapsible : 𝓤 ̇ → 𝓤 ̇
≡-collapsible X = (x y : X) → collapsible(x ≡ y)

sets-are-≡-collapsible : (X : 𝓤 ̇ ) → is-set X → ≡-collapsible X
sets-are-≡-collapsible X s x y = (f , κ)
 where
  f : x ≡ y → x ≡ y
  f p = p
  κ : (p q : x ≡ y) → f p ≡ f q
  κ p q = s x y p q

≡-collapsibles-are-sets : (X : 𝓤 ̇ ) → ≡-collapsible X → is-set X
≡-collapsibles-are-sets X c x = hedberg x (λ y → collapser (x ≡ y) (c x y) ,
                                                 collapser-wconstancy (x ≡ y) (c x y))

subsingletons-are-≡-collapsible : (X : 𝓤 ̇ ) → is-subsingleton X → ≡-collapsible X
subsingletons-are-≡-collapsible X s x y = (f , κ)
 where
  f : x ≡ y → x ≡ y
  f p = s x y
  κ : (p q : x ≡ y) → f p ≡ f q
  κ p q = refl (s x y)

subsingletons-are-sets : (X : 𝓤 ̇ ) → is-subsingleton X → is-set X
subsingletons-are-sets X s = ≡-collapsibles-are-sets X (subsingletons-are-≡-collapsible X s)

subsingletons-are-of-hlevel-1 : (X : 𝓤 ̇ ) → is-subsingleton X → X is-of-hlevel 1
subsingletons-are-of-hlevel-1 X = g
 where
  g : ((x y : X) → x ≡ y) → (x y : X) → is-singleton (x ≡ y)
  g t x y = t x y , subsingletons-are-sets X t x y (t x y)

types-of-hlevel-1-are-subsingletons : (X : 𝓤 ̇ ) → X is-of-hlevel 1 → is-subsingleton X
types-of-hlevel-1-are-subsingletons X = f
 where
  f : ((x y : X) → is-singleton (x ≡ y)) → (x y : X) → x ≡ y
  f s x y = center (x ≡ y) (s x y)

sets-are-of-hlevel-2 : (X : 𝓤 ̇ ) → is-set X → X is-of-hlevel 2
sets-are-of-hlevel-2 X = g
 where
  g : ((x y : X) → is-subsingleton (x ≡ y)) → (x y : X) → (x ≡ y) is-of-hlevel 1
  g t x y = subsingletons-are-of-hlevel-1 (x ≡ y) (t x y)

types-of-hlevel-2-are-sets : (X : 𝓤 ̇ ) → X is-of-hlevel 2 → is-set X
types-of-hlevel-2-are-sets X = f
 where
  f : ((x y : X) → (x ≡ y) is-of-hlevel 1) → (x y : X) → is-subsingleton (x ≡ y)
  f s x y = types-of-hlevel-1-are-subsingletons (x ≡ y) (s x y)

hlevel-upper : (X : 𝓤 ̇ ) (n : ℕ) → X is-of-hlevel n → X is-of-hlevel (succ n)
hlevel-upper X zero = γ
 where
  γ : (h : is-singleton X) (x y : X) → is-singleton (x ≡ y)
  γ h x y = p , subsingletons-are-sets X k x y p
   where
    k : is-subsingleton X
    k = singletons-are-subsingletons X h
    p : x ≡ y
    p = k x y
hlevel-upper X (succ n) = λ h x y → hlevel-upper (x ≡ y) n (h x y)

positive-not-zero : (x : ℕ) → succ x ≢ 0
positive-not-zero x p = 𝟙-is-not-𝟘 (g p)
 where
  f : ℕ → 𝓤₀ ̇
  f 0        = 𝟘
  f (succ x) = 𝟙
  g : succ x ≡ 0 → 𝟙 ≡ 𝟘
  g = ap f

pred : ℕ → ℕ
pred 0 = 0
pred (succ n) = n

succ-lc : {x y : ℕ} → succ x ≡ succ y → x ≡ y
succ-lc = ap pred

ℕ-has-decidable-equality : (x y : ℕ) → (x ≡ y) + (x ≢ y)
ℕ-has-decidable-equality 0 0               = inl (refl 0)
ℕ-has-decidable-equality 0 (succ y)        = inr (≢-sym (positive-not-zero y))
ℕ-has-decidable-equality (succ x) 0        = inr (positive-not-zero x)
ℕ-has-decidable-equality (succ x) (succ y) = f (ℕ-has-decidable-equality x y)
 where
  f : (x ≡ y) + x ≢ y → (succ x ≡ succ y) + (succ x ≢ succ y)
  f (inl p) = inl (ap succ p)
  f (inr k) = inr (λ (s : succ x ≡ succ y) → k (succ-lc s))

ℕ-is-set : is-set ℕ
ℕ-is-set = ≡-collapsibles-are-sets ℕ ℕ-≡-collapsible
 where
  ℕ-≡-collapsible : ≡-collapsible ℕ
  ℕ-≡-collapsible x y = f (ℕ-has-decidable-equality x y) ,
                        κ (ℕ-has-decidable-equality x y)
   where
    f : (x ≡ y) + ¬(x ≡ y) → x ≡ y → x ≡ y
    f (inl p) q = p
    f (inr g) q = !𝟘 (x ≡ y) (g q)
    κ : (d : (x ≡ y) + ¬(x ≡ y)) → wconstant (f d)
    κ (inl p) q r = refl p
    κ (inr g) q r = !𝟘 (f (inr g) q ≡ f (inr g) r) (g q)

has-section : {X : 𝓤 ̇ } {Y : 𝓥 ̇ } → (X → Y) → 𝓤 ⊔ 𝓥 ̇
has-section r = Σ \(s : codomain r → domain r) → r ∘ s ∼ id

_◁_ : 𝓤 ̇ → 𝓥 ̇ → 𝓤 ⊔ 𝓥 ̇
X ◁ Y = Σ \(r : Y → X) → has-section r

retraction : {X : 𝓤 ̇ } {Y : 𝓥 ̇ } → X ◁ Y → Y → X
retraction (r , s , η) = r

section : {X : 𝓤 ̇ } {Y : 𝓥 ̇ } → X ◁ Y → X → Y
section (r , s , η) = s

retract-equation : {X : 𝓤 ̇ } {Y : 𝓥 ̇ } (ρ : X ◁ Y) → retraction ρ ∘ section ρ ∼ 𝑖𝑑 X
retract-equation (r , s , η) = η

◁-refl : (X : 𝓤 ̇ ) → X ◁ X
◁-refl X = 𝑖𝑑 X , 𝑖𝑑 X , refl

_◁∘_ : {X : 𝓤 ̇ } {Y : 𝓥 ̇ } {Z : 𝓦 ̇ } → X ◁ Y → Y ◁ Z → X ◁ Z

(r , s , η) ◁∘ (r' , s' , η') = (r ∘ r' , s' ∘ s , η'')
 where
  η'' = λ x → r (r' (s' (s x))) ≡⟨ ap r (η' (s x)) ⟩
              r (s x)           ≡⟨ η x ⟩
              x                 ∎

_◁⟨_⟩_ : (X : 𝓤 ̇ ) {Y : 𝓥 ̇ } {Z : 𝓦 ̇ } → X ◁ Y → Y ◁ Z → X ◁ Z
X ◁⟨ ρ ⟩ σ = ρ ◁∘ σ

_◀ : (X : 𝓤 ̇ ) → X ◁ X
X ◀ = ◁-refl X

Σ-retract : (X : 𝓤 ̇ ) (A : X → 𝓥 ̇ ) (B : X → 𝓦 ̇ )
          → ((x : X) → (A x) ◁ (B x)) → Σ A ◁ Σ B
Σ-retract X A B ρ = NatΣ r , NatΣ s , η'
 where
  r : (x : X) → B x → A x
  r x = retraction (ρ x)
  s : (x : X) → A x → B x
  s x = section (ρ x)
  η : (x : X) (a : A x) → r x (s x a) ≡ a
  η x = retract-equation (ρ x)
  η' : (σ : Σ A) → NatΣ r (NatΣ s σ) ≡ σ
  η' (x , a) = x , r x (s x a) ≡⟨ ap (λ - → x , -) (η x a) ⟩
               x , a           ∎

Σ-retract-reindexing : {X : 𝓤 ̇ } {Y : 𝓥 ̇ } {A : X → 𝓦 ̇ } (r : Y → X)
                     → has-section r
                     → (Σ \(x : X) → A x) ◁ (Σ \(y : Y) → A (r y))
Σ-retract-reindexing {𝓤} {𝓥} {𝓦} {X} {Y} {A} r (s , η) = γ , φ , γφ
 where
  γ : Σ (A ∘ r) → Σ A
  γ (y , a) = (r y , a)
  φ : Σ A → Σ (A ∘ r)
  φ (x , a) = (s x , transport A ((η x)⁻¹) a)
  γφ : (σ : Σ A) → γ (φ σ) ≡ σ
  γφ (x , a) = to-Σ-≡ (η x , p)
   where
    p = transport A (η x) (transport A ((η x)⁻¹) a) ≡⟨ (ap (λ - → - a) (transport∙ A ((η x)⁻¹) (η x)))⁻¹ ⟩
        transport A ((η x)⁻¹ ∙ η x ) a              ≡⟨ ap (λ - → transport A - a) (⁻¹-left∙ (η x)) ⟩
        transport A (refl x) a                      ≡⟨ refl a ⟩
        a                                           ∎

singleton-type : {X : 𝓤 ̇ } → X → 𝓤 ̇
singleton-type x = Σ \y → y ≡ x

singleton-type-center : {X : 𝓤 ̇ } (x : X) → singleton-type x
singleton-type-center x = (x , refl x)

singleton-type-centered : {X : 𝓤 ̇ } (x y : X) (p : y ≡ x) → singleton-type-center x ≡ (y , p)
singleton-type-centered x x (refl x) = refl (singleton-type-center x)

singleton-types-are-singletons : (X : 𝓤 ̇ ) (x : X) → is-singleton (singleton-type x)
singleton-types-are-singletons X x = singleton-type-center x , φ
 where
  φ : (σ : singleton-type x) → singleton-type-center x ≡ σ
  φ (y , p) = singleton-type-centered x y p

retract-of-singleton : {X : 𝓤 ̇ } {Y : 𝓥 ̇ }
                     → Y ◁ X → is-singleton X → is-singleton Y
retract-of-singleton (r , s , η) (c , φ) = r c , γ
 where
  γ : (y : codomain r) → r c ≡ y
  γ y = r c     ≡⟨ ap r (φ (s y)) ⟩
        r (s y) ≡⟨ η y ⟩
        y       ∎

invertible : {X : 𝓤 ̇ } {Y : 𝓥 ̇ } → (X → Y) → 𝓤 ⊔ 𝓥 ̇
invertible f = Σ \g → (g ∘ f ∼ id) × (f ∘ g ∼ id)

fiber : {X : 𝓤 ̇ } {Y : 𝓥 ̇ } (f : X → Y) → Y → 𝓤 ⊔ 𝓥 ̇
fiber f y = Σ \(x : domain f) → f x ≡ y

fiber-point : {X : 𝓤 ̇ } {Y : 𝓥 ̇ } {f : X → Y} {y : Y}
            → fiber f y → X
fiber-point (x , p) = x

fiberidentification : {X : 𝓤 ̇ } {Y : 𝓥 ̇ } {f : X → Y} {y : Y}
                     → (w : fiber f y) → f (fiber-point w) ≡ y
fiberidentification (x , p) = p

is-equiv : {X : 𝓤 ̇ } {Y : 𝓥 ̇ } → (X → Y) → 𝓤 ⊔ 𝓥 ̇
is-equiv f = (y : codomain f) → is-singleton (fiber f y)

inverse : {X : 𝓤 ̇ } {Y : 𝓥 ̇ } (f : X → Y) → is-equiv f → (Y → X)
inverse f e y = fiber-point (center (fiber f y) (e y))

inverse-is-section : {X : 𝓤 ̇ } {Y : 𝓥 ̇ } (f : X → Y) (e : is-equiv f)
                   → (y : Y) → f (inverse f e y) ≡ y
inverse-is-section f e y = fiberidentification (center (fiber f y) (e y))

inverse-centrality : {X : 𝓤 ̇ } {Y : 𝓥 ̇ } (f : X → Y) (e : is-equiv f) (y : Y)
                   → (t : fiber f y) → (inverse f e y , inverse-is-section f e y) ≡ t
inverse-centrality f e y = centrality (fiber f y) (e y)

inverse-is-retraction : {X : 𝓤 ̇ } {Y : 𝓥 ̇ } (f : X → Y) (e : is-equiv f)
                      → (x : X) → inverse f e (f x) ≡ x
inverse-is-retraction f e x = ap fiber-point p
 where
  p : inverse f e (f x) , inverse-is-section f e (f x) ≡ x , refl (f x)
  p = inverse-centrality f e (f x) (x , (refl (f x)))

equivs-are-invertible : {X : 𝓤 ̇ } {Y : 𝓥 ̇ } (f : X → Y) → is-equiv f → invertible f
equivs-are-invertible f e = (inverse f e , inverse-is-retraction f e , inverse-is-section f e)

invertibles-are-equivs : {X : 𝓤 ̇ } {Y : 𝓥 ̇ } (f : X → Y) → invertible f → is-equiv f
invertibles-are-equivs {𝓤} {𝓥} {X} {Y} f (g , η , ε) y₀ = γ
 where
  a : (y : Y) → (f (g y) ≡ y₀) ◁ (y ≡ y₀)
  a y = r , s , rs
   where
    r : y ≡ y₀ → f (g y) ≡ y₀
    r p = f (g y) ≡⟨ ε y ⟩
          y       ≡⟨ p ⟩
          y₀      ∎
    s : f (g y) ≡ y₀ → y ≡ y₀
    s q = y       ≡⟨ (ε y)⁻¹ ⟩
          f (g y) ≡⟨ q ⟩
          y₀      ∎
    rs : (q : f (g y) ≡ y₀) → r (s q) ≡ q
    rs q = ε y ∙ ((ε y)⁻¹ ∙ q) ≡⟨ (∙assoc (ε y) ((ε y)⁻¹) q)⁻¹ ⟩
           (ε y ∙ (ε y)⁻¹) ∙ q ≡⟨ ap (_∙ q) (⁻¹-right∙ (ε y)) ⟩
           refl (f (g y)) ∙ q  ≡⟨ refl-left ⟩
           q                   ∎
  b : fiber f y₀ ◁ singleton-type y₀
  b = (Σ \(x : X) → f x ≡ y₀)     ◁⟨ Σ-retract-reindexing g (f , η) ⟩
      (Σ \(y : Y) → f (g y) ≡ y₀) ◁⟨ Σ-retract Y (λ y → f (g y) ≡ y₀) (λ y → y ≡ y₀) a ⟩
      (Σ \(y : Y) → y ≡ y₀)       ◀
  γ : is-singleton (fiber f y₀)
  γ = retract-of-singleton b (singleton-types-are-singletons Y y₀)

inverse-is-equiv : {X : 𝓤 ̇ } {Y : 𝓥 ̇ } (f : X → Y) (e : is-equiv f)
                 → is-equiv (inverse f e)
inverse-is-equiv f e = invertibles-are-equivs
                         (inverse f e)
                         (f , inverse-is-section f e , inverse-is-retraction f e)

id-invertible : (X : 𝓤 ̇ ) → invertible (𝑖𝑑 X)
id-invertible X = 𝑖𝑑 X , refl , refl

∘-invertible : {X : 𝓤 ̇ } {Y : 𝓥 ̇ } {Z : 𝓦 ̇ } {f : X → Y} {f' : Y → Z}
             → invertible f' → invertible f → invertible (f' ∘ f)
∘-invertible {𝓤} {𝓥} {𝓦} {X} {Y} {Z} {f} {f'} (g' , gf' , fg') (g , gf , fg)  = g ∘ g' , η , ε
 where
  η : (x : X) → g (g' (f' (f x))) ≡ x
  η x = g (g' (f' (f x))) ≡⟨ ap g (gf' (f x)) ⟩
        g (f x)           ≡⟨ gf x ⟩
        x                 ∎
  ε : (z : Z) → f' (f (g (g' z))) ≡ z
  ε z = f' (f (g (g' z))) ≡⟨ ap f' (fg (g' z)) ⟩
        f' (g' z)         ≡⟨ fg' z ⟩
        z                 ∎

id-is-equiv : (X : 𝓤 ̇ ) → is-equiv (𝑖𝑑 X)
id-is-equiv = singleton-types-are-singletons

∘-is-equiv : {X : 𝓤 ̇ } {Y : 𝓥 ̇ } {Z : 𝓦 ̇ } {f : X → Y} {g : Y → Z}
           → is-equiv g → is-equiv f → is-equiv (g ∘ f)
∘-is-equiv {𝓤} {𝓥} {𝓦} {X} {Y} {Z} {f} {g} i j = γ
 where
  abstract
   γ : is-equiv (g ∘ f)
   γ = invertibles-are-equivs (g ∘ f)
         (∘-invertible (equivs-are-invertible g i)
         (equivs-are-invertible f j))

_≃_ : 𝓤 ̇ → 𝓥 ̇ → 𝓤 ⊔ 𝓥 ̇
X ≃ Y = Σ \(f : X → Y) → is-equiv f

Eq-to-fun : {X : 𝓤 ̇ } {Y : 𝓥 ̇ } → X ≃ Y → X → Y
Eq-to-fun (f , i) = f

Eq-to-fun-is-equiv : {X : 𝓤 ̇ } {Y : 𝓥 ̇ } (e : X ≃ Y) → is-equiv (Eq-to-fun e)
Eq-to-fun-is-equiv (f , i) = i

≃-refl : (X : 𝓤 ̇ ) → X ≃ X
≃-refl X = 𝑖𝑑 X , id-is-equiv X

_●_ : {X : 𝓤 ̇ } {Y : 𝓥 ̇ } {Z : 𝓦 ̇ } → X ≃ Y → Y ≃ Z → X ≃ Z
_●_ {𝓤} {𝓥} {𝓦} {X} {Y} {Z} (f , d) (f' , e) = f' ∘ f , ∘-is-equiv e d

≃-sym : {X : 𝓤 ̇ } {Y : 𝓥 ̇ } → X ≃ Y → Y ≃ X
≃-sym (f , e) = inverse f e , inverse-is-equiv f e

_≃⟨_⟩_ : (X : 𝓤 ̇ ) {Y : 𝓥 ̇ } {Z : 𝓦 ̇ } → X ≃ Y → Y ≃ Z → X ≃ Z
_ ≃⟨ d ⟩ e = d ● e

_■ : (X : 𝓤 ̇ ) → X ≃ X
_■ = ≃-refl

transport-is-equiv : {X : 𝓤 ̇ } (A : X → 𝓥 ̇ ) {x y : X} (p : x ≡ y)
                   → is-equiv (transport A p)
transport-is-equiv A (refl x) = id-is-equiv (A x)

transport-≃ : {X : 𝓤 ̇ } (A : X → 𝓥 ̇ ) {x y : X}
            → x ≡ y → A x ≃ A y
transport-≃ A p = transport A p , transport-is-equiv A p

ap' : {X : 𝓤 ̇ } (A : X → 𝓥 ̇ ) {x y : X}
    → x ≡ y → A x ≡ A y
ap' = ap

transport-is-equiv' : {X : 𝓤 ̇ } (A : X → 𝓥 ̇ ) {x y : X} (p : x ≡ y)
                    → is-equiv (transport A p)
transport-is-equiv' A p =
  invertibles-are-equivs
   (transport A p)
   (transport A (p ⁻¹) ,
    (λ a → transport A (p ⁻¹) (transport A p a) ≡⟨ (ap (λ - → - a) (transport∙ A p (p ⁻¹)))⁻¹ ⟩
           transport A (p ∙ p ⁻¹) a             ≡⟨ ap (λ - → transport A - a) (⁻¹-right∙ p) ⟩
           a                                    ∎) ,
     λ a → transport A p (transport A (p ⁻¹) a) ≡⟨ (ap (λ - → - a) (transport∙ A (p ⁻¹) p))⁻¹ ⟩
           transport A (p ⁻¹ ∙ p) a             ≡⟨ ap (λ - → transport A - a) (⁻¹-left∙ p) ⟩
           a                                    ∎)

Σ-≡-equiv : {X : 𝓤 ̇ } {A : X → 𝓥 ̇ } (σ τ : Σ A)
          → (σ ≡ τ) ≃ (Σ \(p : pr₁ σ ≡ pr₁ τ) → pr₂ σ ≡[ p / A ] pr₂ τ)
Σ-≡-equiv  {𝓤} {𝓥} {X} {A}  σ τ = from-Σ-≡ ,
                                  invertibles-are-equivs from-Σ-≡ (to-Σ-≡ , ε , η)
 where
  η : (w : Σ \(p : pr₁ σ ≡ pr₁ τ) → transport A p (pr₂ σ) ≡ pr₂ τ) → from-Σ-≡ (to-Σ-≡ w) ≡ w
  η (refl p , refl q) = refl (refl p , refl q)
  ε : (q : σ ≡ τ) → to-Σ-≡ (from-Σ-≡ q) ≡ q
  ε (refl σ) = refl (refl σ)

Id-to-Eq : (X Y : 𝓤 ̇ ) → X ≡ Y → X ≃ Y
Id-to-Eq X X (refl X) = ≃-refl X

is-univalent : (𝓤 : Universe) → 𝓤 ⁺ ̇
is-univalent 𝓤 = (X Y : 𝓤 ̇ ) → is-equiv (Id-to-Eq X Y)

Eq-to-Id : is-univalent 𝓤 → (X Y : 𝓤 ̇ ) → X ≃ Y → X ≡ Y
Eq-to-Id ua X Y = inverse (Id-to-Eq X Y) (ua X Y)

Id-to-fun : {X Y : 𝓤 ̇ } → X ≡ Y → X → Y
Id-to-fun {𝓤} {X} {Y} p = Eq-to-fun (Id-to-Eq X Y p)

Id-to-funs-agree : {X Y : 𝓤 ̇ } (p : X ≡ Y)
                 → Id-to-fun p ≡ Id-to-Fun p
Id-to-funs-agree (refl X) = refl (𝑖𝑑 X)

H-≃ : is-univalent 𝓤
    → (X : 𝓤 ̇ ) (A : (Y : 𝓤 ̇ ) → X ≃ Y → 𝓥 ̇ )
    → A X (≃-refl X) → (Y : 𝓤 ̇ ) (e : X ≃ Y) → A Y e
H-≃ {𝓤} {𝓥} ua X A a Y e = γ
 where
  A' : (Y : 𝓤 ̇ ) → X ≡ Y → 𝓥 ̇
  A' Y p = A Y (Id-to-Eq X Y p)
  a' : A' X (refl X)
  a' = a
  f' : (Y : 𝓤 ̇ ) (p : X ≡ Y) → A' Y p
  f' = H X A' a'
  g : A Y (Id-to-Eq X Y (Eq-to-Id ua X Y e))
  g = f' Y (Eq-to-Id ua X Y e)
  p : Id-to-Eq X Y (Eq-to-Id ua X Y e) ≡ e
  p = inverse-is-section (Id-to-Eq X Y) (ua X Y) e
  γ : A Y e
  γ = transport (A Y) p g

J-≃ : is-univalent 𝓤
    → (A : (X Y : 𝓤 ̇ ) → X ≃ Y → 𝓥 ̇ )
    → ((X : 𝓤 ̇) → A X X (≃-refl X))
    → (X Y : 𝓤 ̇ ) (e : X ≃ Y) → A X Y e
J-≃ ua A φ X = H-≃ ua X (A X) (φ X)

H-equiv : is-univalent 𝓤
        → (X : 𝓤 ̇ ) (A : (Y : 𝓤 ̇ ) → (X → Y) → 𝓥 ̇ )
        → A X (𝑖𝑑 X) → (Y : 𝓤 ̇ ) (f : X → Y) → is-equiv f → A Y f
H-equiv {𝓤} {𝓥} ua X A a Y f i = γ (f , i) i
 where
  B : (Y : 𝓤 ̇ ) → X ≃ Y → 𝓤 ⊔ 𝓥 ̇
  B Y (f , i) = is-equiv f → A Y f
  b : B X (≃-refl X)
  b = λ (_ : is-equiv (𝑖𝑑 X)) → a
  γ : (e : X ≃ Y) → B Y e
  γ = H-≃ ua X B b Y

J-equiv : is-univalent 𝓤
        → (A : (X Y : 𝓤 ̇ ) → (X → Y) → 𝓥 ̇ )
        → ((X : 𝓤 ̇ ) → A X X (𝑖𝑑 X))
        → (X Y : 𝓤 ̇ ) (f : X → Y) → is-equiv f → A X Y f
J-equiv ua A φ X = H-equiv ua X (A X) (φ X)

J-invertible : is-univalent 𝓤
             → (A : (X Y : 𝓤 ̇ ) → (X → Y) → 𝓥 ̇ )
             → ((X : 𝓤 ̇ ) → A X X (𝑖𝑑 X))
             → (X Y : 𝓤 ̇ ) (f : X → Y) → invertible f → A X Y f
J-invertible ua A φ X Y f i = J-equiv ua A φ X Y f (invertibles-are-equivs f i)

Σ-change-of-variables : is-univalent 𝓤
                      → (X : 𝓤 ̇ ) (P : X → 𝓥 ̇) (Y : 𝓤 ̇) (f : X → Y)
                      → (i : is-equiv f)
                      → (Σ \(x : X) → P x) ≡ (Σ \(y : Y) → P (inverse f i y))
Σ-change-of-variables {𝓤} {𝓥} ua X P Y f i = H-≃ ua X A a Y (f , i)
 where
   A : (Y : 𝓤 ̇) → X ≃ Y →  (𝓤 ⊔ 𝓥) ⁺ ̇
   A Y (f , i) = (Σ P) ≡ (Σ (P ∘ inverse f i))
   a : A X (≃-refl X)
   a = refl (Σ P)

Σ-change-of-variables' : is-univalent 𝓤
                       → (X : 𝓤 ̇ ) (P : X → 𝓥 ̇) (Y : 𝓤 ̇) (g : Y → X)
                       → (i : is-equiv g)
                       → (Σ \(x : X) → P x) ≡ (Σ \(y : Y) → P (g y))
Σ-change-of-variables' {𝓤} {𝓥} ua X P Y g j = Σ-change-of-variables ua X P Y
                                                 (inverse g j)
                                                 (inverse-is-equiv g j)

is-hae : {X : 𝓤 ̇ } {Y : 𝓥 ̇ } → (X → Y) → 𝓤 ⊔ 𝓥 ̇
is-hae f = Σ \(g : codomain f → domain f)
         → Σ \(η : g ∘ f ∼ id)
         → Σ \(ε : f ∘ g ∼ id)
         → (x : domain f) → ap f (η x) ≡ ε (f x)

haes-are-invertible : {X Y : 𝓤 ̇ } (f : X → Y)
                    → is-hae f → invertible f
haes-are-invertible f (g , η , ε , _) = g , η , ε

id-is-hae : (X : 𝓤 ̇ ) → is-hae (𝑖𝑑 X)
id-is-hae X = 𝑖𝑑 X , refl , refl , (λ x → refl (refl x))

invertibles-are-haes : is-univalent 𝓤
                     → (X Y : 𝓤 ̇ ) (f : X → Y)
                     → invertible f → is-hae f
invertibles-are-haes ua = J-invertible ua (λ X Y f → is-hae f) id-is-hae

swap₂ : 𝟚 → 𝟚
swap₂ ₀ = ₁
swap₂ ₁ = ₀

swap₂-involutive : (n : 𝟚) → swap₂ (swap₂ n) ≡ n
swap₂-involutive ₀ = refl ₀
swap₂-involutive ₁ = refl ₁

swap₂-is-equiv : is-equiv swap₂
swap₂-is-equiv = invertibles-are-equivs swap₂ (swap₂ , swap₂-involutive , swap₂-involutive)

e₀ e₁ : 𝟚 ≃ 𝟚
e₀ = ≃-refl 𝟚
e₁ = swap₂ , swap₂-is-equiv

e₀-is-not-e₁ : e₀ ≢ e₁
e₀-is-not-e₁ p = ₁-is-not-₀ r
 where
  q : id ≡ swap₂
  q = ap Eq-to-fun p
  r : ₁ ≡ ₀
  r = ap (λ - → - ₁) q

module _ (ua : is-univalent 𝓤₀) where

  p₀ p₁ : 𝟚 ≡ 𝟚
  p₀ = Eq-to-Id ua 𝟚 𝟚 e₀
  p₁ = Eq-to-Id ua 𝟚 𝟚 e₁

  p₀-is-not-p₁ : p₀ ≢ p₁
  p₀-is-not-p₁ q = e₀-is-not-e₁ r
   where
    r = e₀              ≡⟨ (inverse-is-section (Id-to-Eq 𝟚 𝟚) (ua 𝟚 𝟚) e₀)⁻¹ ⟩
        Id-to-Eq 𝟚 𝟚 p₀ ≡⟨ ap (Id-to-Eq 𝟚 𝟚) q ⟩
        Id-to-Eq 𝟚 𝟚 p₁ ≡⟨ inverse-is-section (Id-to-Eq 𝟚 𝟚) (ua 𝟚 𝟚) e₁ ⟩
        e₁              ∎

  𝓤₀-is-not-a-set :  ¬(is-set (𝓤₀ ̇ ))
  𝓤₀-is-not-a-set s = p₀-is-not-p₁ q
   where
    q : p₀ ≡ p₁
    q = s 𝟚 𝟚 p₀ p₁

left-cancellable : {X : 𝓤 ̇ } {Y : 𝓥 ̇ } → (X → Y) → 𝓤 ⊔ 𝓥 ̇
left-cancellable f = {x x' : domain f} → f x ≡ f x' → x ≡ x'

lc-maps-reflect-subsingletonness : {X : 𝓤 ̇ } {Y : 𝓥 ̇ } (f : X → Y)
                                 → left-cancellable f
                                 → is-subsingleton Y
                                 → is-subsingleton X

has-retraction : {X : 𝓤 ̇ } {Y : 𝓥 ̇ } → (X → Y) → 𝓤 ⊔ 𝓥 ̇
has-retraction s = Σ \(r : codomain s → domain s) → r ∘ s ∼ id

sections-are-lc : {X : 𝓤 ̇ } {A : 𝓥 ̇ } (s : X → A) → has-retraction s → left-cancellable s

equivs-have-retractions : {X : 𝓤 ̇ } {Y : 𝓥 ̇ } (f : X → Y) → is-equiv f → has-retraction f

equivs-have-sections : {X : 𝓤 ̇ } {Y : 𝓥 ̇ } (f : X → Y) → is-equiv f → has-section f

equivs-are-lc : {X : 𝓤 ̇ } {Y : 𝓥 ̇ } (f : X → Y) → is-equiv f → left-cancellable f

equiv-to-subsingleton : {X : 𝓤 ̇ } {Y : 𝓥 ̇ } (f : X → Y)
                      → is-equiv f
                      → is-subsingleton Y
                      → is-subsingleton X

equiv-to-subsingleton' : {X : 𝓤 ̇ } {Y : 𝓥 ̇ } (f : X → Y)
                       → is-equiv f
                       → is-subsingleton X
                       → is-subsingleton Y

sections-closed-under-∼ : {X : 𝓤 ̇ } {Y : 𝓥 ̇ } (f g : X → Y)
                        → has-retraction f
                        → g ∼ f
                        → has-retraction g

retractions-closed-under-∼ : {X : 𝓤 ̇ } {Y : 𝓥 ̇ } (f g : X → Y)
                           → has-section f
                           → g ∼ f
                           → has-section g

is-joyal-equiv : {X : 𝓤 ̇ } {Y : 𝓥 ̇ } → (X → Y) → 𝓤 ⊔ 𝓥 ̇
is-joyal-equiv f = has-section f × has-retraction f

joyal-equivs-are-invertible : {X : 𝓤 ̇ } {Y : 𝓥 ̇ } (f : X → Y)
                            → is-joyal-equiv f → invertible f

joyal-equivs-are-equivs : {X : 𝓤 ̇ } {Y : 𝓥 ̇ } (f : X → Y)
                        → is-joyal-equiv f → is-equiv f

invertibles-are-joyal-equivs : {X : 𝓤 ̇ } {Y : 𝓥 ̇ } (f : X → Y)
                             → invertible f → is-joyal-equiv f

equivs-are-joyal-equivs : {X : 𝓤 ̇ } {Y : 𝓥 ̇ } (f : X → Y)
                        → is-equiv f → is-joyal-equiv f

equivs-closed-under-∼ : {X : 𝓤 ̇ } {Y : 𝓥 ̇ } (f g : X → Y)
                      → is-equiv f
                      → g ∼ f
                      → is-equiv g

equivs-closed-under-∼' : {X : 𝓤 ̇ } {Y : 𝓥 ̇ } (f g : X → Y)
                       → is-equiv f
                       → f ∼ g
                       → is-equiv g

≃-gives-◁ : (X : 𝓤 ̇ ) (Y : 𝓥 ̇ ) → X ≃ Y → X ◁ Y

≃-gives-▷ : (X : 𝓤 ̇ ) (Y : 𝓥 ̇ ) → X ≃ Y → Y ◁ X

equiv-to-singleton : (X : 𝓤 ̇ ) (Y : 𝓥 ̇ )
                   → X ≃ Y → is-singleton Y → is-singleton X

equiv-to-singleton' : (X : 𝓤 ̇ ) (Y : 𝓥 ̇ )
                    → X ≃ Y → is-singleton X → is-singleton Y

subtypes-of-sets-are-sets : {X : 𝓤 ̇ } {Y : 𝓥 ̇ } (m : X → Y)
                          → left-cancellable m → is-set Y → is-set X

pr₁-lc : {X : 𝓤 ̇ } {A : X → 𝓥 ̇ } → ((x : X) → is-subsingleton (A x))
       → left-cancellable  (λ (t : Σ A) → pr₁ t)

subsets-of-sets-are-sets : (X : 𝓤 ̇ ) (A : X → 𝓥 ̇ )
                         → is-set X
                         → ((x : X) → is-subsingleton(A x))
                         → is-set(Σ \(x : X) → A x)

pr₁-equivalence : (X : 𝓤 ̇ ) (A : X → 𝓥 ̇ )
                → ((x : X) → is-singleton (A x))
                → is-equiv (λ (t : Σ A) → pr₁ t)

ΠΣ-distr-≃ : {X : 𝓤 ̇ } {A : X → 𝓥 ̇ } {P : (x : X) → A x → 𝓦 ̇ }
           → (Π \(x : X) → Σ \(a : A x) → P x a) ≃ (Σ \(f : Π A) → Π \(x : X) → P x (f x))

Σ-cong : {X : 𝓤 ̇ } {A : X → 𝓥 ̇ } {B : X → 𝓦 ̇ }
       → ((x : X) → A x ≃ B x) → Σ A ≃ Σ B

⁻¹-≃ : {X : 𝓤 ̇ } (x y : X) → (x ≡ y) ≃ (y ≡ x)

singleton-type' : {X : 𝓤 ̇ } → X → 𝓤 ̇
singleton-type' x = Σ \y → x ≡ y

singleton-types-≃ : {X : 𝓤 ̇ } (x : X) → singleton-type' x ≃ singleton-type x

singleton-types-are-singletons' : (X : 𝓤 ̇ ) (x : X) → is-singleton (singleton-type' x)

singletons-equivalent : (X : 𝓤 ̇ ) (Y : 𝓥 ̇ )
                      → is-singleton X → is-singleton Y → X ≃ Y

maps-of-singletons-are-equivs : (X : 𝓤 ̇ ) (Y : 𝓥 ̇ ) (f : X → Y)
                              → is-singleton X → is-singleton Y → is-equiv f

logically-equivalent-subsingletons-are-equivalent : (X : 𝓤 ̇ ) (Y : 𝓥 ̇ )
                                                  → is-subsingleton X
                                                  → is-subsingleton Y
                                                  → X ⇔ Y
                                                  → X ≃ Y

NatΣ-fiber-equiv : {X : 𝓤 ̇ } (A : X → 𝓥 ̇ ) (B : X → 𝓦 ̇ ) (φ : Nat A B)
                 → (x : X) (b : B x) → fiber (φ x) b ≃ fiber (NatΣ φ) (x , b)

NatΣ-equiv-gives-fiberwise-equiv : {X : 𝓤 ̇ } (A : X → 𝓥 ̇ ) (B : X → 𝓦 ̇ ) (φ : Nat A B)
                                 → is-equiv (NatΣ φ) → ((x : X) → is-equiv (φ x))

Σ-is-subsingleton : {X : 𝓤 ̇ } {A : X → 𝓥 ̇ }
                  → is-subsingleton X
                  → ((x : X) → is-subsingleton (A x))
                  → is-subsingleton (Σ A)

×-is-subsingleton : {X : 𝓤 ̇ } {Y : 𝓥 ̇ }
                  → is-subsingleton X
                  → is-subsingleton Y
                  → is-subsingleton (X × Y)

to-×-≡ : {X : 𝓤 ̇ } {Y : 𝓥 ̇ } {z t : X × Y}
       → pr₁ z ≡ pr₁ t
       → pr₂ z ≡ pr₂ t
       → z ≡ t

×-is-subsingleton' : {X : 𝓤 ̇ } {Y : 𝓥 ̇ }
                   → ((Y → is-subsingleton X) × (X → is-subsingleton Y))
                   → is-subsingleton (X × Y)

×-is-subsingleton'-back : {X : 𝓤 ̇ } {Y : 𝓥 ̇ }
                        → is-subsingleton (X × Y)
                        → (Y → is-subsingleton X) × (X → is-subsingleton Y)

ap₂ : {X : 𝓤 ̇ } {Y : 𝓥 ̇ } {Z : 𝓦 ̇ } (f : X → Y → Z) {x x' : X} {y y' : Y}
    → x ≡ x' → y ≡ y' → f x y ≡ f x' y'

infix  0 _◁_
infix  1 _◀
infixr 0 _◁⟨_⟩_
infix  0 _≃_
infixl 2 _●_
infixr 0 _≃⟨_⟩_
infix  1 _■

lc-maps-reflect-subsingletonness f l s x x' = l (s (f x) (f x'))

sections-are-lc s (r , ε) {x} {y} p = x       ≡⟨ (ε x)⁻¹ ⟩
                                      r (s x) ≡⟨ ap r p ⟩
                                      r (s y) ≡⟨ ε y ⟩
                                      y       ∎

equivs-have-retractions f e = (inverse f e , inverse-is-retraction f e)

equivs-have-sections f e = (inverse f e , inverse-is-section f e)

equivs-are-lc f e = sections-are-lc f (equivs-have-retractions f e)

equiv-to-subsingleton f e = lc-maps-reflect-subsingletonness f (equivs-are-lc f e)

equiv-to-subsingleton' f e = lc-maps-reflect-subsingletonness
                               (inverse f e)
                               (equivs-are-lc (inverse f e) (inverse-is-equiv f e))

sections-closed-under-∼ f g (r , rf) h = (r ,
                                          λ x → r (g x) ≡⟨ ap r (h x) ⟩
                                                r (f x) ≡⟨ rf x ⟩
                                                x       ∎)

retractions-closed-under-∼ f g (s , fs) h = (s ,
                                             λ y → g (s y) ≡⟨ h (s y) ⟩
                                                   f (s y) ≡⟨ fs y ⟩
                                                   y ∎)

joyal-equivs-are-invertible f ((s , fs) , (r , rf)) = (s , sf , fs)
 where
  sf = λ (x : domain f) → s(f x)       ≡⟨ (rf (s (f x)))⁻¹ ⟩
                          r(f(s(f x))) ≡⟨ ap r (fs (f x)) ⟩
                          r(f x)       ≡⟨ rf x ⟩
                          x            ∎

joyal-equivs-are-equivs f j = invertibles-are-equivs f (joyal-equivs-are-invertible f j)

invertibles-are-joyal-equivs f (g , gf , fg) = ((g , fg) , (g , gf))

equivs-are-joyal-equivs f e = invertibles-are-joyal-equivs f (equivs-are-invertible f e)

equivs-closed-under-∼ f g e h =
 joyal-equivs-are-equivs g
  (retractions-closed-under-∼ f g (equivs-have-sections    f e) h ,
   sections-closed-under-∼    f g (equivs-have-retractions f e) h)

equivs-closed-under-∼' f g e h = equivs-closed-under-∼ f g e (λ x → (h x)⁻¹)

≃-gives-◁ X Y (f , e) = (inverse f e , f , inverse-is-retraction f e)

≃-gives-▷ X Y (f , e) = (f , inverse f e , inverse-is-section f e)

equiv-to-singleton X Y e = retract-of-singleton (≃-gives-◁ X Y e)

equiv-to-singleton' X Y e = retract-of-singleton (≃-gives-▷ X Y e)

subtypes-of-sets-are-sets {𝓤} {𝓥} {X} m i h = ≡-collapsibles-are-sets X c
 where
  f : (x x' : X) → x ≡ x' → x ≡ x'
  f x x' r = i (ap m r)
  κ : (x x' : X) (r s : x ≡ x') → f x x' r ≡ f x x' s
  κ x x' r s = ap i (h (m x) (m x') (ap m r) (ap m s))
  c : ≡-collapsible X
  c x x' = f x x' , κ x x'

pr₁-lc i p = to-Σ-≡ (p , i _ _ _)

subsets-of-sets-are-sets X A h p = subtypes-of-sets-are-sets pr₁ (pr₁-lc p) h

pr₁-equivalence {𝓤} {𝓥} X A s = invertibles-are-equivs pr₁ (g , η , ε)
 where
  g : X → Σ A
  g x = x , pr₁(s x)
  ε : (x : X) → pr₁ (g x) ≡ x
  ε x = refl (pr₁ (g x))
  η : (σ : Σ A) → g (pr₁ σ) ≡ σ
  η (x , a) = to-Σ-≡ (ε x , singletons-are-subsingletons (A x) (s x) _ a)

ΠΣ-distr-≃ {𝓤} {𝓥} {𝓦} {X} {A} {P} = φ , invertibles-are-equivs φ (γ , η , ε)
 where
  φ : (Π \(x : X) → Σ \(a : A x) → P x a) → Σ \(f : Π A) → Π \(x : X) → P x (f x)
  φ g = ((λ x → pr₁ (g x)) , λ x → pr₂ (g x))

  γ : (Σ \(f : Π A) → Π \(x : X) → P x (f x)) → Π \(x : X) → Σ \(a : A x) → P x a
  γ (f , φ) x = f x , φ x
  η : γ ∘ φ ∼ id
  η = refl
  ε : φ ∘ γ ∼ id
  ε = refl

Σ-cong {𝓤} {𝓥} {𝓦} {X} {A} {B} φ =
  (NatΣ f , invertibles-are-equivs (NatΣ f) (NatΣ g , NatΣ-η , NatΣ-ε))
 where
  f : (x : X) → A x → B x
  f x = Eq-to-fun (φ x)
  g : (x : X) → B x → A x
  g x = inverse (f x) (Eq-to-fun-is-equiv (φ x))
  η : (x : X) (a : A x) → g x (f x a) ≡ a
  η x = inverse-is-retraction (f x) (Eq-to-fun-is-equiv (φ x))
  ε : (x : X) (b : B x) → f x (g x b) ≡ b
  ε x = inverse-is-section (f x) (Eq-to-fun-is-equiv (φ x))

  NatΣ-η : (w : Σ A) → NatΣ g (NatΣ f w) ≡ w
  NatΣ-η (x , a) = x , g x (f x a) ≡⟨ ap (λ - → x , -) (η x a) ⟩
                   x , a           ∎

  NatΣ-ε : (t : Σ B) → NatΣ f (NatΣ g t) ≡ t
  NatΣ-ε (x , b) = x , f x (g x b) ≡⟨ ap (λ - → x , -) (ε x b) ⟩
                   x , b           ∎

⁻¹-≃ x y = (_⁻¹ , invertibles-are-equivs _⁻¹ (_⁻¹ , ⁻¹-involutive , ⁻¹-involutive))

singleton-types-≃ x = Σ-cong (λ y → ⁻¹-≃ x y)

singleton-types-are-singletons' X x = equiv-to-singleton
                                       (singleton-type' x)
                                       (singleton-type x)
                                       (singleton-types-≃ x)
                                       (singleton-types-are-singletons X x)

singletons-equivalent X Y i j = f , invertibles-are-equivs f (g , η , ε)
 where
  f : X → Y
  f x = center Y j
  g : Y → X
  g y = center X i
  η : (x : X) → g (f x) ≡ x
  η = centrality X i
  ε : (y : Y) → f (g y) ≡ y
  ε = centrality Y j

maps-of-singletons-are-equivs X Y f i j = invertibles-are-equivs f (g , η , ε)
 where
  g : Y → X
  g y = center X i
  η : (x : X) → g (f x) ≡ x
  η = centrality X i
  ε : (y : Y) → f (g y) ≡ y
  ε y = singletons-are-subsingletons Y j (f (g y)) y

logically-equivalent-subsingletons-are-equivalent X Y i j (f , g) =
  f , invertibles-are-equivs f (g , (λ x → i (g (f x)) x) , (λ y → j (f (g y)) y))

NatΣ-fiber-equiv A B φ x b = (f , invertibles-are-equivs f (g , ε , η))
 where
  f : fiber (φ x) b → fiber (NatΣ φ) (x , b)
  f (a , refl _) = ((x , a) , refl (x , φ x a))
  g : fiber (NatΣ φ) (x , b) → fiber (φ x) b
  g ((x , a) , refl _) = (a , refl (φ x a))
  ε : (w : fiber (φ x) b) → g (f w) ≡ w
  ε (a , refl _) = refl (a , refl (φ x a))
  η : (t : fiber (NatΣ φ) (x , b)) → f (g t) ≡ t
  η ((x , a) , refl _) = refl ((x , a) , refl (NatΣ φ (x , a)))

NatΣ-equiv-gives-fiberwise-equiv A B φ e x b = γ
 where
  γ : is-singleton (fiber (φ x) b)
  γ = equiv-to-singleton
         (fiber (φ x) b)
         (fiber (NatΣ φ) (x , b))
         (NatΣ-fiber-equiv A B φ x b)
         (e (x , b))

Σ-is-subsingleton i j (x , a) (y , b) = to-Σ-≡ (i x y , j y _ _)

×-is-subsingleton i j = Σ-is-subsingleton i (λ _ → j)

to-×-≡ (refl x) (refl y) = refl (x , y)

×-is-subsingleton' {𝓤} {𝓥} {X} {Y} (i , j) = k
 where
  k : is-subsingleton (X × Y)
  k (x , y) (x' , y') = to-×-≡ (i y x x') (j x y y')

×-is-subsingleton'-back {𝓤} {𝓥} {X} {Y} k = i , j
 where
  i : Y → is-subsingleton X
  i y x x' = ap pr₁ (k (x , y) (x' , y))
  j : X → is-subsingleton Y
  j x y y' = ap pr₂ (k (x , y) (x , y'))

ap₂ f (refl x) (refl y) = refl (f x y)

