---
layout: default
title : Introduction to Univalent Foundations of Mathematics with Agda
date : 2019-03-04
---
## <a name="lecturenotes">Introduction to Univalent Foundations of Mathematics with Agda</a>

<!--
\begin{code}
{-# OPTIONS --without-K --exact-split --safe #-}

module FunExt where

open import Universes
open import MLTT-Agda
open import HoTT-UF-Agda
\end{code}
-->

[<sub>Table of contents ⇑</sub>](toc.html#contents)
### <a name="funextfromua"></a> Function extensionality from univalence

Function extensionality says that any two pointwise equal functions
are equal. This is known to be not provable or disprovable in
MLTT. It is an independent statement, which we abbreviate as `funext`.

\begin{code}
funext : ∀ 𝓤 𝓥 → (𝓤 ⊔ 𝓥)⁺ ̇
funext 𝓤 𝓥 = {X : 𝓤 ̇ } {Y : 𝓥 ̇ } {f g : X → Y} → f ∼ g → f ≡ g
\end{code}

There [will be](FunExt.html#hfunext) two stronger statements, namely
the generalization to dependent functions, and the requirement that
the canonical map `(f ≡ g) → (f ∼ g) ` is an equivalence.

*Exercise.* Assuming `funext`, prove that, if `f : X → Y` is an equivalence
then so is the function `(-) ∘ f : (Y → Z) → (X → Z)`.

The crucial step in [Voevodsky's proof](http://www.math.uwo.ca/faculty/kapulkin/notes/ua_implies_fe.pdf) that univalence implies funext
is to establish the conclusion of the above exercise assuming
univalence instead.  This relies on the following lemma, which
describes pre-composition of equivalences in terms of `transport`.

\begin{code}
transport-is-pre-comp : (ua : is-univalent 𝓤) {X Y Z : 𝓤 ̇ } (e : X ≃ Y) (g : Y → Z)
                      → transport (λ - → - → Z) ((Eq-to-Id ua X Y e)⁻¹) g ≡ g ∘ Eq-to-fun e
\end{code}

We will use this with `e = (f , i)` and `i : is-equiv f`, in which
case `Eq-to-fun e` is `f`, as the function `Eq-to-fun : X ≃ Y → X → Y`
is defined to be the first projection.

In order to be able to proceed by `≡-induction` on an identification
`p : X ≡ Y`, we define the auxiliary function `α`, and then take `p`
to be `Eq-to-Id ua X Y e`.

\begin{code}
transport-is-pre-comp ua {X} {Y} {Z} e g = α e (Eq-to-Id ua X Y e) (refl (Eq-to-Id ua X Y e))
 where
  α : (e : X ≃ Y) (p : X ≡ Y)
    → p ≡ Eq-to-Id ua X Y e
    → transport (λ - → - → Z) (p ⁻¹) g ≡ g ∘ Eq-to-fun e
  α e (refl X) = γ
   where
    γ : refl X ≡ Eq-to-Id ua X X e → g ≡ g ∘ Eq-to-fun e
    γ q = ap (g ∘_) b
     where
      a : ≃-refl X ≡ e
      a = ≃-refl X                         ≡⟨ ap (Id-to-Eq X X) q ⟩
          Id-to-Eq X X (Eq-to-Id ua X X e) ≡⟨ inverse-is-section (Id-to-Eq X X) (ua X X) e ⟩
          e                                ∎
      b : id ≡ Eq-to-fun e
      b = ap Eq-to-fun a
\end{code}

The following is then an immediate consequence of the above lemma,
using the facts that transports are equivalences and that equivalences
are closed under pointwise equality.

\begin{code}
pre-comp-is-equiv : (ua : is-univalent 𝓤) {X Y Z : 𝓤 ̇ } (f : X → Y)
                  → is-equiv f
                  → is-equiv (λ (g : Y → Z) → g ∘ f)
pre-comp-is-equiv ua {X} {Y} {Z} f i = j
 where
  e : X ≃ Y
  e = (f , i)

  of-course : Eq-to-fun e ≡ f
  of-course = refl f

  φ γ : (Y → Z) → (X → Z)
  φ g = g ∘ f
  γ g = transport (λ - → - → Z) ((Eq-to-Id ua X Y e)⁻¹) g

  γ-is-equiv : is-equiv γ
  γ-is-equiv = transport-is-equiv (λ - → - → Z) ((Eq-to-Id ua X Y e)⁻¹)

  h' : (g : Y → Z) → transport (λ - → - → _) ((Eq-to-Id ua X Y e)⁻¹) g ≡ g ∘ Eq-to-fun e
  h' = transport-is-pre-comp ua e

  h : γ ∼ φ
  h = h'

  j : is-equiv φ
  j = equivs-closed-under-∼' γ φ γ-is-equiv h
\end{code}

A cryptic version of the above proof is the following:

\begin{code}
pre-comp-is-equiv' : (ua : is-univalent 𝓤) {X Y Z : 𝓤 ̇ } (f : X → Y)
                   → is-equiv f
                   → is-equiv (λ (g : Y → Z) → g ∘ f)
pre-comp-is-equiv' ua {X} {Y} {Z} f i =
 equivs-closed-under-∼'
  (transport (λ - → - → Z) ((Eq-to-Id ua X Y (f , i))⁻¹))
  (_∘ f)
  (transport-is-equiv (λ - → - → Z) ((Eq-to-Id ua X Y (f , i))⁻¹))
  (transport-is-pre-comp ua (f , i))
\end{code}

With this we can prove the desired result as follows.

\begin{code}
univalence-gives-funext : is-univalent 𝓤 → funext 𝓥 𝓤
univalence-gives-funext ua {X} {Y} {f₀} {f₁} h = γ
 where
  Δ = Σ \(y₀ : Y) → Σ \(y₁ : Y) → y₀ ≡ y₁

  δ : Y → Δ
  δ y = (y , y , refl y)

  π₀ π₁ : Δ → Y
  π₀ (y₀ , y₁ , p) = y₀
  π₁ (y₀ , y₁ , p) = y₁

  δ-is-equiv : is-equiv δ
  δ-is-equiv = invertibles-are-equivs δ (π₀ , η , ε)
   where
    η : (y : Y) → π₀ (δ y) ≡ y
    η y = refl y
    ε : (d : Δ) → δ (π₀ d) ≡ d
    ε (y , y , refl y) = refl (y , y , refl y)

  πδ : π₀ ∘ δ ≡ π₁ ∘ δ
  πδ = refl id

  φ : (Δ → Y) → (Y → Y)
  φ π = π ∘ δ

  φ-is-equiv : is-equiv φ
  φ-is-equiv = pre-comp-is-equiv ua δ δ-is-equiv

  π₀-equals-π₁ : π₀ ≡ π₁
  π₀-equals-π₁ = equivs-are-lc φ φ-is-equiv πδ

  γ : f₀ ≡ f₁
  γ = ap (λ π x → π (f₀ x , f₁ x , h x)) π₀-equals-π₁
\end{code}

This definition of `γ` is probably too quick. Here are all the steps
performed silently by Agda, by expanding judgmental equalities,
indicated with `refl` here:

\begin{code}
  γ' = f₀                              ≡⟨ refl _ ⟩
       (λ x → f₀ x)                    ≡⟨ refl _ ⟩
       (λ x → π₀ (f₀ x , f₁ x , h x))  ≡⟨ ap (λ π x → π (f₀ x , f₁ x , h x)) π₀-equals-π₁ ⟩
       (λ x → π₁ (f₀ x , f₁ x , h x))  ≡⟨ refl _ ⟩
       (λ x → f₁ x)                    ≡⟨ refl _ ⟩
       f₁                              ∎
\end{code}

So notice that this relies on the so-called η-rule for judgmental
equality of functions, namely `f = λ x → f x`. Without it, we would
only get that

   > `f₀ ∼ f₁ → (λ x → f₀ x) ≡ (λ x → f₁ x)`

instead.

[<sub>Table of contents ⇑</sub>](toc.html#contents)
### <a name="hfunext"></a> Variations of function extensionality and their logical equivalence

Dependent function extensionality:

\begin{code}
dfunext : ∀ 𝓤 𝓥 → 𝓤 ⁺ ⊔ 𝓥 ⁺ ̇
dfunext 𝓤 𝓥 = {X : 𝓤 ̇ } {A : X → 𝓥 ̇ } {f g : Π A} → f ∼ g → f ≡ g
\end{code}

The above says that there is some map `f ~ g → f ≡ g`. The following
instead says that the canonical map in the other direction is an
equivalence:

\begin{code}
happly : {X : 𝓤 ̇ } {A : X → 𝓥 ̇ } (f g : Π A) → f ≡ g → f ∼ g
happly f g p x = ap (λ - → - x) p

hfunext : ∀ 𝓤 𝓥 → (𝓤 ⊔ 𝓥)⁺ ̇
hfunext 𝓤 𝓥 = {X : 𝓤 ̇ } {A : X → 𝓥 ̇ } (f g : Π A) → is-equiv (happly f g)

hfunext-gives-dfunext : hfunext 𝓤 𝓥 → dfunext 𝓤 𝓥
hfunext-gives-dfunext hfe {X} {A} {f} {g} = inverse (happly f g) (hfe f g)
\end{code}

Voevodsky showed that all notions of function extensionaliry are
logically equivalent to saying that products of singletons are
singletons:

\begin{code}
vvfunext : ∀ 𝓤 𝓥 → 𝓤 ⁺ ⊔ 𝓥 ⁺ ̇
vvfunext 𝓤 𝓥 = {X : 𝓤 ̇ } {A : X → 𝓥 ̇ } → ((x : X) → is-singleton (A x)) → is-singleton (Π A)

dfunext-gives-vvfunext : dfunext 𝓤 𝓥 → vvfunext 𝓤 𝓥
dfunext-gives-vvfunext fe {X} {A} i = f , c
 where
  f : Π A
  f x = center (A x) (i x)
  c : (g : Π A) → f ≡ g
  c g = fe (λ (x : X) → centrality (A x) (i x) (g x))
\end{code}

We need some lemmas to get `hfunext` from `vvfunext`:

\begin{code}
post-comp-is-invertible : {X : 𝓤 ̇ } {Y : 𝓥 ̇ } {A : 𝓦 ̇ }
                        → funext 𝓦 𝓤 → funext 𝓦 𝓥
                        → (f : X → Y) → invertible f → invertible (λ (h : A → X) → f ∘ h)
post-comp-is-invertible {𝓤} {𝓥} {𝓦} {X} {Y} {A} nfe nfe' f (g , η , ε) = (g' , η' , ε')
 where
  f' : (A → X) → (A → Y)
  f' h = f ∘ h
  g' : (A → Y) → (A → X)
  g' k = g ∘ k
  η' : (h : A → X) → g' (f' h) ≡ h
  η' h = nfe (η ∘ h)
  ε' : (k : A → Y) → f' (g' k) ≡ k
  ε' k = nfe' (ε ∘ k)

post-comp-is-equiv : {X : 𝓤 ̇ } {Y : 𝓥 ̇ } {A : 𝓦 ̇ } → funext 𝓦 𝓤 → funext 𝓦 𝓥
                   → (f : X → Y) → is-equiv f → is-equiv (λ (h : A → X) → f ∘ h)
post-comp-is-equiv fe fe' f e = invertibles-are-equivs
                                 (λ h → f ∘ h)
                                 (post-comp-is-invertible fe fe' f (equivs-are-invertible f e))

vvfunext-gives-hfunext : vvfunext 𝓤 𝓥 → hfunext 𝓤 𝓥
vvfunext-gives-hfunext {𝓤} {𝓥} vfe {X} {Y} f = γ
 where
  a : (x : X) → is-singleton (Σ \(y : Y x) → f x ≡ y)
  a x = singleton-types-are-singletons' (Y x) (f x)
  c : is-singleton ((x : X) → Σ \(y : Y x) → f x ≡ y)
  c = vfe a
  R : (Σ \(g : Π Y) → f ∼ g) ◁ (Π \(x : X) → Σ \(y : Y x) → f x ≡ y)
  R = ≃-gives-▷ _ _ ΠΣ-distr-≃
  r : (Π \(x : X) → Σ \(y : Y x) → f x ≡ y) → Σ \(g : Π Y) → f ∼ g
  r = λ _ → f , (λ x → refl (f x))
  d : is-singleton (Σ \(g : Π Y) → f ∼ g)
  d = retract-of-singleton R c
  e : (Σ \(g : Π Y) → f ≡ g) → (Σ \(g : Π Y) → f ∼ g)
  e = NatΣ (happly f)
  i : is-equiv e
  i = maps-of-singletons-are-equivs (Σ (λ g → f ≡ g)) (Σ (λ g → f ∼ g)) e
       (singleton-types-are-singletons' (Π Y) f) d
  γ : (g : Π Y) → is-equiv (happly f g)
  γ = NatΣ-equiv-gives-fiberwise-equiv (λ g → f ≡ g) (λ g → f ∼ g) (happly f) i
\end{code}

And finally the seemingly rather weak, non-dependent version `funext`
implies the seemingly strongest version, which closes the circle of
logical equivalences.

\begin{code}
funext-gives-vvfunext : funext 𝓤 (𝓤 ⊔ 𝓥) → funext 𝓤 𝓤 → vvfunext 𝓤 𝓥
funext-gives-vvfunext {𝓤} {𝓥} fe fe' {X} {A} φ = γ
  where
   f : Σ A → X
   f = pr₁
   f-is-equiv : is-equiv f
   f-is-equiv = pr₁-equivalence X A φ
   g : (X → Σ A) → (X → X)
   g h = f ∘ h
   g-is-equiv : is-equiv g
   g-is-equiv = post-comp-is-equiv fe fe' f f-is-equiv
   i : is-singleton (Σ \(h : X → Σ A) → f ∘ h ≡ id)
   i = g-is-equiv id
   r : (Σ \(h : X → Σ A) → f ∘ h ≡ id) → Π A
   r (h , p) x = transport A (happly (f ∘ h) id p x) (pr₂ (h x))
   s : Π A → (Σ \(h : X → Σ A) → f ∘ h ≡ id)
   s φ = (λ x → x , φ x) , refl id
   rs : ∀ φ → r (s φ) ≡ φ
   rs φ = refl (r (s φ))
   γ : is-singleton (Π A)
   γ = retract-of-singleton (r , s , rs) i
\end{code}

Corollaries:

\begin{code}
funext-gives-hfunext : funext 𝓤 (𝓤 ⊔ 𝓥) → funext 𝓤 𝓤 → hfunext 𝓤 𝓥
funext-gives-hfunext fe fe' = vvfunext-gives-hfunext (funext-gives-vvfunext fe fe')

funext-gives-dfunext : funext 𝓤 (𝓤 ⊔ 𝓥) → funext 𝓤 𝓤 → dfunext 𝓤 𝓥
funext-gives-dfunext fe fe' = hfunext-gives-dfunext (funext-gives-hfunext fe fe')

univalence-gives-hfunext' : is-univalent 𝓤 → is-univalent (𝓤 ⊔ 𝓥) → hfunext 𝓤 𝓥
univalence-gives-hfunext' ua ua' = funext-gives-hfunext
                                     (univalence-gives-funext ua')
                                     (univalence-gives-funext ua)

univalence-gives-vvfunext' : is-univalent 𝓤 → is-univalent (𝓤 ⊔ 𝓥) → vvfunext 𝓤 𝓥
univalence-gives-vvfunext' ua ua' = funext-gives-vvfunext
                                     (univalence-gives-funext ua')
                                     (univalence-gives-funext ua)

univalence-gives-hfunext : is-univalent 𝓤 → hfunext 𝓤 𝓤
univalence-gives-hfunext ua = univalence-gives-hfunext' ua ua

univalence-gives-dfunext : is-univalent 𝓤 → dfunext 𝓤 𝓤
univalence-gives-dfunext ua = hfunext-gives-dfunext (univalence-gives-hfunext ua)

univalence-gives-vvfunext : is-univalent 𝓤 → vvfunext 𝓤 𝓤
univalence-gives-vvfunext ua = univalence-gives-vvfunext' ua ua
\end{code}

[<sub>Table of contents ⇑</sub>](toc.html#contents)
### <a name="univalencesubsingleton"></a> The univalence axiom is a subsingleton type

If we use a type as an axiom, it should better have at most one element. We
prove some generally useful lemmas first.

\begin{code}
Π-is-subsingleton : dfunext 𝓤 𝓥 → {X : 𝓤 ̇ } {A : X → 𝓥 ̇ }
                  → ((x : X) → is-subsingleton (A x))
                  → is-subsingleton (Π A)
Π-is-subsingleton fe i f g = fe (λ x → i x (f x) (g x))

being-a-singleton-is-a-subsingleton : dfunext 𝓤 𝓤 → {X : 𝓤 ̇ }
                                    → is-subsingleton (is-singleton X)
being-a-singleton-is-a-subsingleton fe {X} (x , φ) (y , γ) = p
 where
  i : is-subsingleton X
  i = singletons-are-subsingletons X (y , γ)
  s : is-set X
  s = subsingletons-are-sets X i
  p : (x , φ) ≡ (y , γ)
  p = to-Σ-≡ (φ y , fe (λ (z : X) → s y z _ _))

being-an-equiv-is-a-subsingleton : dfunext 𝓥 (𝓤 ⊔ 𝓥) → dfunext (𝓤 ⊔ 𝓥) (𝓤 ⊔ 𝓥)
                                 → {X : 𝓤 ̇ } {Y : 𝓥 ̇ } (f : X → Y)
                                 → is-subsingleton (is-equiv f)
being-an-equiv-is-a-subsingleton fe fe' f =
 Π-is-subsingleton fe (λ x → being-a-singleton-is-a-subsingleton fe')

univalence-is-a-subsingleton : is-univalent (𝓤 ⁺) → is-subsingleton (is-univalent 𝓤)
univalence-is-a-subsingleton {𝓤} ua⁺ ua ua' = p
 where
  fe₀  : funext 𝓤 𝓤
  fe₁  : funext 𝓤 (𝓤 ⁺)
  fe₂  : funext (𝓤 ⁺) (𝓤 ⁺)
  dfe₁ : dfunext 𝓤 (𝓤 ⁺)
  dfe₂ : dfunext (𝓤 ⁺) (𝓤 ⁺)
  fe₀  = univalence-gives-funext ua
  fe₁  = univalence-gives-funext ua⁺
  fe₂  = univalence-gives-funext ua⁺
  dfe₁ = funext-gives-dfunext fe₁ fe₀
  dfe₂ = funext-gives-dfunext fe₂ fe₂

  i : is-subsingleton (is-univalent 𝓤)
  i = Π-is-subsingleton dfe₂
       (λ X → Π-is-subsingleton dfe₂
               (λ Y → being-an-equiv-is-a-subsingleton dfe₁ dfe₂ (Id-to-Eq X Y)))

  p : ua ≡ ua'
  p = i ua ua'
\end{code}

So if all universes are univalent then "being univalent" is a
subsingleton, and hence a singleton. This hypothesis of global
univalence cannot be expressed in our MLTT that only has `ω`
many universes, because global univalence would have to live in the
first universe after them. Agda does have such a universe `𝓤ω,` and so
we can formulate it here. There would be no problem in extending our
MLTT to have such a universe if we so wished, in which case we would
be able to formulate and prove:

\begin{code}
global-univalence : 𝓤ω
global-univalence = ∀ 𝓤 → is-univalent 𝓤

univalence-is-a-subsingletonω : global-univalence → is-subsingleton (is-univalent 𝓤)
univalence-is-a-subsingletonω {𝓤} γ = univalence-is-a-subsingleton (γ (𝓤 ⁺))

univalence-is-a-singleton : global-univalence → is-singleton (is-univalent 𝓤)
univalence-is-a-singleton {𝓤} γ = pointed-subsingletons-are-singletons
                                   (is-univalent 𝓤)
                                   (γ 𝓤)
                                   (univalence-is-a-subsingletonω γ)
\end{code}

That the type `global-univalence` would be a subsingleton can't even be formulated in
the absence of a universe of level `ω + 1`.

In the absence of a universe `𝓤ω` in our MLTT, we can simply have an
axiom scheme, consisting of `ω`-many axioms, stating that each
universe is univalent. Then we can prove in our MLTT that the univalence property
for each inverse is a (sub)singleton, with `ω`-many proofs.

[<sub>Table of contents ⇑</sub>](toc.html#contents)
### <a name="hfunextsubsingleton"></a> `hfunext` and `vvfunext` are subsingletons

This is left as an exercise. Like univalence, the proof that these two
forms of function extensional extensionality require assumptions of
function extensionality at higher universes. So perhaps it is more
convenient to just assume global univalence. An inconvenience is that
the natural tool to use, Π-is-subsingleton, needs products with
explicit arguments, but we made some of the arguments of hfunext and
vvfunext implicit. One way around this problem is to define equivalent
versions with the arguments explicit, and establish an equivalence
between the new version and the original version.

[<sub>Table of contents ⇑</sub>](toc.html#contents)
### <a name="morefunextuses"></a> More applications of function extensionality

\begin{code}
being-a-subsingleton-is-a-subsingleton : {X : 𝓤 ̇ } → dfunext 𝓤 𝓤
                                       → is-subsingleton (is-subsingleton X)
being-a-subsingleton-is-a-subsingleton {𝓤} {X} fe i j = c
 where
  l : is-set X
  l = subsingletons-are-sets X i
  a : (x y : X) → i x y ≡ j x y
  a x y = l x y (i x y) (j x y)
  b : (x : X) → i x ≡ j x
  b x = fe (a x)
  c : i ≡ j
  c = fe b
\end{code}

Here is a situation where `hfunext` is what is needed:

\begin{code}
Π-is-set : hfunext 𝓤 𝓥 → {X : 𝓤 ̇ } {A : X → 𝓥 ̇ }
         → ((x : X) → is-set(A x)) → is-set(Π A)
Π-is-set hfe s f g = b
 where
  a : is-subsingleton (f ∼ g)
  a p q = hfunext-gives-dfunext hfe ((λ x → s x (f x) (g x) (p x) (q x)))
  b : is-subsingleton(f ≡ g)
  b = equiv-to-subsingleton (happly f g) (hfe f g) a

being-set-is-a-subsingleton : dfunext 𝓤 𝓤 → {X : 𝓤 ̇ } → is-subsingleton (is-set X)
being-set-is-a-subsingleton {𝓤} fe {X} =
 Π-is-subsingleton fe
   (λ x → Π-is-subsingleton fe
           (λ y → being-a-subsingleton-is-a-subsingleton fe))
\end{code}

More generally:

\begin{code}
hlevel-relation-is-subsingleton : dfunext 𝓤 𝓤
                                → (n : ℕ) (X : 𝓤 ̇ ) → is-subsingleton (X is-of-hlevel n)
hlevel-relation-is-subsingleton {𝓤} fe zero     X = being-a-singleton-is-a-subsingleton fe
hlevel-relation-is-subsingleton {𝓤} fe (succ n) X =
  Π-is-subsingleton fe
    (λ x → Π-is-subsingleton fe
            (λ x' → hlevel-relation-is-subsingleton {𝓤} fe n (x ≡ x')))
\end{code}

Composition of equivalences is associative:

\begin{code}
●-assoc : dfunext 𝓣 (𝓤 ⊔ 𝓣) → dfunext (𝓤 ⊔ 𝓣) (𝓤 ⊔ 𝓣)
        → {X : 𝓤 ̇ } {Y : 𝓥 ̇ } {Z : 𝓦 ̇ } {T : 𝓣 ̇ }
          (α : X ≃ Y) (β : Y ≃ Z) (γ : Z ≃ T)
        → α ● (β ● γ) ≡ (α ● β) ● γ
●-assoc fe fe' (f , a) (g , b) (h , c) = ap (h ∘ g ∘ f ,_) q
 where
  d e : is-equiv (h ∘ g ∘ f)
  d = ∘-is-equiv (∘-is-equiv c b) a
  e = ∘-is-equiv c (∘-is-equiv b a)

  q : d ≡ e
  q = being-an-equiv-is-a-subsingleton fe fe' (h ∘ g ∘ f) _ _

inversion-involutive : {X : 𝓤 ̇ } {Y : 𝓥 ̇ } (f : X → Y) (e : is-equiv f)
                     → inverse (inverse f e) (inverse-is-equiv f e) ≡ f
inversion-involutive f e = refl f

≃-sym-involutive : dfunext 𝓥 (𝓤 ⊔ 𝓥) → dfunext (𝓥 ⊔ 𝓤) (𝓥 ⊔ 𝓤) →
                   {X : 𝓤 ̇ } {Y : 𝓥 ̇ } (α : X ≃ Y)
                 → ≃-sym (≃-sym α) ≡ α
≃-sym-involutive fe fe' (f , a) = to-Σ-≡ (inversion-involutive f a ,
                                          being-an-equiv-is-a-subsingleton fe fe' f _ _)
\end{code}

*Exercise.* The hlevels are closed under `Σ` and, using `hfunext`, also
under `Π`. Univalence is not needed, but makes the proof easier.  (If
you don't use univalence, you will need to show that hlevels are
closed under equivalence.)

[<sub>Table of contents ⇑</sub>](toc.html#contents) [<sub> Subsingleton truncation ⇓ </sub>](Inhabitation.html)
